5 - Un interpréteur pour le langage While

Interp.v
@@ -13,7 +13,30 @@ Require Import WhileBigStep.
 Require Import Lia.
 
 Fixpoint exec_prog (fuel: nat) (env: state) (i: stmt) : option state :=
-None.
+  match fuel with
+  | O => None
+  | S fuel_1 =>
+    match i with
+    | Skip => Some env
+    | Assign v e => Some (update_state env v (eval_expr env e))
+    | Seq s1 s2 =>
+      match exec_prog fuel_1 env s1 with
+      | None => None
+      | Some env' => exec_prog fuel_1 env' s2
+      end
+    | If c s1 s2 => 
+      if eval_cond env c
+      then exec_prog fuel_1 env s1
+      else exec_prog fuel_1 env s2
+    | While c Inv s =>
+      if eval_cond env c
+      then match exec_prog fuel_1 env s with
+      | None => None
+      | Some env' => exec_prog fuel_1 env' (While c Inv s)
+      end
+      else Some env
+    end
+  end.
 
 Definition p1 :=
   Seq
@@ -38,7 +61,35 @@ Compute
 Theorem exec_prog_bigstep:
   forall fuel s i s', exec_prog fuel s i = Some s' -> bigstep s i s'.
 Proof.
-Admitted.
+  intro.
+  induction fuel.
+  - intros. simpl in H. discriminate H.
+  - intros. destruct i.
+    * injection H as H. rewrite H. apply bigstep_skip.
+    * injection H as H. rewrite <- H. apply bigstep_assign.
+    * destruct (exec_prog fuel s i1) eqn:Eqn.
+      -- eapply bigstep_seq.
+        ** eapply IHfuel. apply Eqn.
+        ** eapply IHfuel. simpl in H. rewrite Eqn in H. apply H.
+      -- eapply bigstep_seq.
+        ** eapply IHfuel. simpl in H. rewrite Eqn in H. rewrite <- H. apply Eqn.
+        ** eapply IHfuel. simpl in H. rewrite Eqn in H. rewrite <- H. discriminate.
+    * simpl in H. destruct (eval_cond s c) eqn:E2.
+      -- eapply bigstep_if_true.
+        ** apply eval_cond_true. apply E2.
+        ** apply IHfuel. apply H.
+      -- eapply bigstep_if_false.
+        ** apply eval_cond_false. apply E2.
+        ** apply IHfuel. apply H.
+    * simpl in H. destruct (eval_cond s c) eqn:E3. destruct (exec_prog fuel s i) eqn:E4.
+      -- eapply bigstep_while_true.
+        ** apply eval_cond_true. apply E3.
+        ** apply IHfuel. eapply E4.
+        ** apply IHfuel. apply H.
+      -- discriminate.
+      -- injection H as H. rewrite <- H. eapply bigstep_while_false. apply eval_cond_false. apply E3.
+Qed.
+
 
 Lemma exec_prog_more_fuel:
   forall f s i s',
@@ -46,12 +97,76 @@ Lemma exec_prog_more_fuel:
   -> forall f', f' >= f
   -> exec_prog f' s i = Some s'.
 Proof.
-Admitted.
+  intros fuel.
+  induction fuel.
+  - intros. inversion H.
+  - intros. simpl in H.  destruct f'.
+  * lia.
+  * simpl. destruct i.
+    -- apply H.
+    -- apply H.
+    -- destruct (exec_prog fuel s i1) eqn:E.
+      ** eapply IHfuel in E. 
+        --- rewrite E. eapply IHfuel in H.
+          *** eapply H.
+          *** lia.
+        --- lia.
+      ** discriminate.
+    -- destruct (eval_cond s c) eqn:E2.
+      ** eapply IHfuel.
+        --- apply H.
+        --- lia.
+      ** eapply IHfuel.
+        --- apply H.
+        --- lia.
+    -- destruct (eval_cond s c) eqn:E3.
+      ** destruct (exec_prog fuel s i) eqn:E4.
+        --- eapply IHfuel in E4.
+          *** rewrite E4. eapply IHfuel.
+            ---- apply H.
+            ---- lia.
+          *** lia.
+        --- discriminate.
+      ** congruence.
+Qed.
 
 Theorem bigstep_exec_prog:
   forall s i s',
   bigstep s i s'
   -> exists fuel, exec_prog fuel s i = Some s'.
 Proof.
-Admitted.
-
+  intros s i s' H.
+  induction H.
+  - exists 1. simpl. reflexivity.
+  - exists 1. simpl. reflexivity.
+  - destruct IHbigstep1. destruct IHbigstep2. exists (S (max x x0)). simpl.
+  rewrite (exec_prog_more_fuel x env s1 env').
+    * rewrite (exec_prog_more_fuel x0 env' s2 env'').
+      + reflexivity.
+      + apply H2.
+      + lia.
+    * apply H1.
+    * lia.
+  - destruct IHbigstep as [fuel]. exists (S fuel). simpl.
+  destruct (eval_cond env c) eqn:E2.
+    * apply H1.
+    * apply eval_cond_true in H. congruence.
+  - destruct IHbigstep as [fuel]. exists (S fuel). simpl.
+  destruct (eval_cond env c) eqn:E3.
+    * apply eval_cond_false in H. congruence.
+    * apply H1.
+  - apply eval_cond_false in H. exists 1. simpl.
+  destruct (eval_cond env c) eqn:E4.
+    * discriminate.
+    * reflexivity.
+  - destruct IHbigstep1 as [fuel1]. destruct IHbigstep2 as [fuel2].
+  exists (S (max fuel1 fuel2)). simpl. destruct (eval_cond env c) eqn:E5.
+    * apply eval_cond_true in H. rewrite (exec_prog_more_fuel fuel1 env s env').
+      + rewrite (exec_prog_more_fuel fuel2 env' (While c I s) env'').
+        -- reflexivity.
+        -- apply H3.
+        -- lia.
+      + apply H2.
+      + lia.
+    * apply eval_cond_true in H. congruence.
+Qed.
